\documentclass[11pt,letterpaper]{article}                  % Define document class

%! Mandatory packages
\usepackage[utf8]{inputenc}                                %! Character encoding
\usepackage[T1]{fontenc}                                   %! Font encoding
\usepackage[english]{babel}                                %! Language setting

% Set path
\newcommand{\path}{/Users/Attila/OneDrive - Duke University/texts/latex-sample/Preamble}

% Text packages
\input{"\path/packText.tex"}

% Figure/table packages
\input{"\path/packFigure.tex"}

% Math packages
\input{"\path/packMath.tex"}

% Graphics packages
\input{"\path/packGraph.tex"}

% Title
\title{Replication study}
\author{\Large Jackson Bunting and Attila Gyetvai\footnote{Department of Economics, Duke University. Emails: \href{mailto:jackson.bunting@duke.edu}{jackson.bunting@duke.edu}, \href{mailto:attila.gyetvai@duke.edu}{attila.gyetvai@duke.edu}. All errors are ours.}}
\date{\today}


%%%%%%%%%%%%%%%%%%%%%%%%%%%%%%%%%

\begin{document}

\maketitle

\section{Framework}

Following \citet{Blomquist2002}.

\begin{align*}
	h_i^* &\equiv \pi (y_i, w_i, v_i); \\
	\bar{\pi} (y_i, w_i) &\equiv \int \pi(y_i, w_i, v_i) g(v_i) \, d v_i; \\
	\mu(y_i, w_i, \ell_i) &= \int_{-\infty}^{\pi^{-1}(y_i, w_i, \ell_i)} \left[ \pi (y_i, w_i, v_i) - \ell_i \right] g(v_i) \, d v_i.
\end{align*}

\section{A simple example}

Suppose that an individual $i$ is endowed with $y_i$ nonlabor income and 1 unit of time, which she can divide between work $h_i$ and leisure $1-h_i$.
Therefore she can spend up to $y_i + w_i h_i$ where $w_i$ is her wage rate.
Assume for the moment that her budget set is linear; we introduce nonlinearities in a moment.

Individual $i$'s preferences towards consumption $c_i$ and work $h_i$ can be represented by a Cobb-Douglas utility function; consequently the optimization problem she faces is 
\begin{align*}
	\max_{c_i, h_i} \enskip c_i^{1-v_i} (1-h_i)^{v_i} \qquad \text{s.t.} \enskip c_i \leq y_i + w_i h_i
\end{align*}
where $v_i$ is an unknown scalar specific to $i$.
The resulting labor supply function is
\begin{align*}
	h^*_i &\equiv \pi (y_i, w_i, v_i) = 1 - \frac{(1-v_i) y_i}{w_i}.\footnotemark
\end{align*}
\footnotetext{Calculations can be found in Appendix \ref{app:CD}.}
We calculate
\begin{align*}
	\bar{\pi} (y_i, w_i) &= 1 - \frac{y_i}{2 w_i} \qquad \text{and} \\
\end{align*}


\section{Estimation}

\begin{align*}
	\hat{h}(x) &= p^K (x)' \hat{\beta} \\
	p^K (x)' &= \begin{pmatrix}
		\left[ y_J^{p(k)} w_J^{q(k)} \right] ' \\
		\left[ \sum_{j=1}^{J-1} \left( \ell_j^{m(k)} y_j^{p(k)} w_j^{q(k)} - \ell_j^{m(k)} y_{j+1}^{p(k)} w_{j+1}^{q(k)} \right) \right]'
	\end{pmatrix}
\end{align*}

\bibliographystyle{apalike}
\bibliography{project}

\appendix

\section{Cobb-Douglas utility}
\label{app:CD}

The maximization problem can be equivalently written as
\begin{align*}
	&\max_{h_i} \enskip (y_i + w_i h_i)^{1-v_i} (1-h_i)^{v_i}.
	\intertext{The first-order condition is}
	0 &= (1-v_i) (y_i + w_i h_i^*)^{-v_i} w_i (1-h_i^*)^{v_i} + v_i (y_i + w_i h_i^*)^{1-v_i} (1-h_i^*)^{v_i-1} \cdot (-1) \\
	  &= (1-v_i) w_i (1-h_i^*) - v_i (y_i + w_i h_i^*) \\
	  &= (1-v_i) w_i - (1-v_i) w_i h_i^* - v_i y_i - v_i w_i h_i^* \\
	  &= (1-v_i) w_i - w_i h_i^* - v_i y_i.
	\intertext{Rearranging yields}
	h_i^* &\equiv \pi (y_i, w_i, v_i) = 1 - v_i - \frac{v_i y_i}{w_i}.
\end{align*}
We get $\bar{\pi}_i (y_i, w_i)$ by integrating $v_i$ out:
\begin{align*}
	\bar{\pi}_i (y_i, w_i) &= \int_0^1 1 - v_i - \frac{v_i y_i}{w_i} \, d v_i = \left[ v_i - \frac{v_i^2}{2} - \frac{v_i^2 y_i}{2 w_i} \right]_{v_i=0}^1 = \frac{1}{2} - \frac{y_i}{2 w_i}.
	\intertext{Furthermore, we calculate the inverse of $\pi$ w.r.t $v_i$ as follows:}
	\ell_i &= 1 - v_i - \frac{v_i y_i}{w_i} \\
	w_i \ell_i &= w_i - v_i w_i - v_i y_i = w_i - v_i (w_i + y_i) \\
	v_i (w_i + y_i) &= w_i - w_i \ell_i = w_i (1-\ell_i) \\
	v_i &= \frac{w_i (1-\ell_i)}{w_i + y_i} \equiv \pi^{-1} (y_i, w_i, \ell_i)
	\intertext{Finally, we derive $\mu (y_i, w_i, \ell_i)$ as}
	\mu (y_i, w_i, \ell_i) &= \int_0^{\frac{w_i (1-\ell_i)}{w_i + y_i}} 1 - v_i - \frac{v_i y_i}{w_i} - \ell_i \, d v_i \\
	&= \left[ v_i - \frac{v_i^2}{2} - \frac{v_i^2 y_i}{2 w_i} - \ell_i v_i \right]_{v_i = 0}^{\frac{w_i (1-\ell_i)}{w_i + y_i}} \\
	&= \left[ (1-\ell_i) v_i - \frac{v_i^2}{2} \left( 1 + \frac{y_i}{w_i} \right) \right]_{v_i = 0}^{\frac{w_i (1-\ell_i)}{w_i + y_i}} \\
	&= \left[ (1-\ell_i) v_i - \frac{v_i^2}{2} \frac{w_i + y_i}{w_i} \right]_{v_i = 0}^{\frac{w_i (1-\ell_i)}{w_i + y_i}} \\
	&= \frac{w_i (1-\ell_i)^2}{w_i + y_i} - \frac{w_i^2 (1-\ell_i)^2}{2 (w_i + y_i)^2} \frac{w_i + y_i}{w_i} \\
	&= \frac{w_i (1-\ell_i)^2}{2 (w_i + y_i)}
\end{align*}

\end{document}








